Matching (hopefully) complete

src/Quantifiers/directory.lean
@@ -30,21 +30,46 @@ meta structure entry : Type :=
 (edeps : list expr) -- expression dependancies, e.g. P x
 (build_stack : build_stack) -- data for use at build time
 
-meta def directory := rbmap expr entry expr.lt_prop
+open tactic expr native
+
+meta def directory := rb_map expr entry
+
+meta def get_side (dir : directory) (key : expr) : tactic side :=
+match dir.find key with
+| some e := return e.side
+| none   := failed
+end
+
+meta def get_ldeps (dir : directory) (key : expr) : tactic (list expr) :=
+match dir.find key with
+| some e := return e.ldeps
+| none   := failed
+end
+
+meta def get_edeps (dir : directory) (key : expr) : tactic (list expr) :=
+match dir.find key with
+| some e := return e.edeps
+| none   := failed
+end
+
+meta def get_build_stack (dir : directory) (key : expr) : tactic build_stack :=
+match dir.find key with
+| some e := return e.build_stack
+| none   := failed
+end
 
 meta def goals := list expr
 
-open tactic expr
 meta def new_mvar (tp : expr): tactic expr :=
 do nm ← mk_fresh_name,
   (num : fin 1000) ← random,  -- create quasi-unique display name to aid debugging
   let disp_nm := ("m" ++ to_string (num : ℕ) : name),
   return (mvar nm disp_nm tp)
 
-meta def get_edeps : expr → tactic (list expr)
+meta def find_edeps : expr → tactic (list expr)
 | (app f x) :=
-do l₁ ← get_edeps f,
-  l₂ ← get_edeps x,
+do l₁ ← find_edeps f,
+  l₂ ← find_edeps x,
   return (l₁ ++ l₂)
 | (mvar nm₁ nm₂ tp) := return [mvar nm₁ nm₂ tp] 
 | _ := return []
@@ -57,24 +82,24 @@ meta def process_local : expr → directory → list expr → build_stack → ta
 | `(Exists (λ x : %%tp, %%rest)) dir ldeps bs :=
 do f ← to_expr ``(λ x : %%tp, %%rest),
   new_key ← new_mvar tp,
-  edeps ← get_edeps tp,
+  edeps ← find_edeps tp,
   let new_bs := (list.cons (build_type.ass_ex, new_key) bs.1, bs.2),
-  let new_dir := rbmap.insert dir new_key ⟨given, ldeps, edeps, new_bs⟩,
+  let new_dir := rb_map.insert dir new_key ⟨given, ldeps, edeps, new_bs⟩,
   recursion_expr ← whnf (app f new_key),
   process_local recursion_expr new_dir ldeps new_bs
 | `(∀ x : %%tp, %%rest) dir ldeps bs := 
 do f ← to_expr ``(λ x : %%tp, %%rest),
   new_key ← new_mvar tp,
-  edeps ← get_edeps tp,
+  edeps ← find_edeps tp,
   let new_bs := (list.cons (build_type.ass_all, new_key) bs.1, bs.2),
-  let new_dir := rbmap.insert dir new_key ⟨choose, [], edeps, new_bs⟩,
+  let new_dir := rb_map.insert dir new_key ⟨choose, [], edeps, new_bs⟩,
   recursion_expr ← whnf (app f new_key),
   process_local recursion_expr new_dir (list.cons new_key ldeps) new_bs
 | single dir ldeps bs :=
 do new_key ← new_mvar single,
-  edeps ← get_edeps single,
+  edeps ← find_edeps single,
   let new_bs := (list.cons (build_type.ass_atom, new_key) bs.1, bs.2),
-  return $ rbmap.insert dir new_key ⟨given, ldeps, edeps, new_bs⟩
+  return $ rb_map.insert dir new_key ⟨given, ldeps, edeps, new_bs⟩
 
 meta def process_goal : expr → goals → directory → list expr → build_stack → tactic (directory × goals)
 -- first argument is the relevant local constant
@@ -85,29 +110,29 @@ meta def process_goal : expr → goals → directory → list expr → build_sta
 | `(Exists (λ x : %%tp, %%rest)) gls dir ldeps bs := 
 do f ← to_expr ``(λ x : %%tp, %%rest),
   new_key ← new_mvar tp,
-  edeps ← get_edeps tp,
+  edeps ← find_edeps tp,
   let new_bs := (list.cons (build_type.goal_ex, new_key) bs.1, bs.2),
-  let new_dir := rbmap.insert dir new_key ⟨choose, [], edeps, new_bs⟩,
+  let new_dir := rb_map.insert dir new_key ⟨choose, [], edeps, new_bs⟩,
   recursion_expr ← whnf (app f new_key),
   process_goal recursion_expr gls new_dir (list.cons new_key ldeps) new_bs
 | `(∀ x : %%tp, %%rest) gls dir ldeps bs := 
 do f ← to_expr ``(λ x : %%tp, %%rest),
   new_key ← new_mvar tp,
-  edeps ← get_edeps tp,
+  edeps ← find_edeps tp,
   let new_bs := (list.cons (build_type.goal_all, new_key) bs.1, bs.2),
-  let new_dir := rbmap.insert dir new_key ⟨given, ldeps, edeps, new_bs⟩,
+  let new_dir := rb_map.insert dir new_key ⟨given, ldeps, edeps, new_bs⟩,
   recursion_expr ← whnf (app f new_key),
   process_goal recursion_expr (list.cons new_key gls) new_dir ldeps new_bs
 | single gls dir ldeps bs := 
 do new_key ← new_mvar single,
-  edeps ← get_edeps single,
+  edeps ← find_edeps single,
   let new_bs := (list.cons (build_type.goal_atom, new_key) bs.1, bs.2),
-  return (rbmap.insert dir new_key ⟨choose, [], edeps, new_bs⟩, list.cons new_key gls)
+  return (rb_map.insert dir new_key ⟨choose, [], edeps, new_bs⟩, list.cons new_key gls)
 
 meta def create_directory : tactic (directory × goals) :=
 do ctx ← local_context,
   tgt ← target,
-  let dir : directory := mk_rbmap expr entry expr.lt_prop,
+  let dir : directory := rb_map.mk expr entry,
   ctx.foldl
     (λ tdir h,
     do dir ← tdir,
