src/Quantifiers/matching_test.lean
@@ -1,0 +1,31 @@
+import Quantifiers.matching
+
+universe u
+
+open tactic
+
+example {α : Type u} (a : α) : α :=
+by do (dir, goals) ← create_directory,
+  mi ← create_match_info dir goals,
+  trace_match_info mi, -- the important line
+
+  ta ← get_local `a,
+  exact ta
+
+example {α : Type u} (P : α → Prop) (Q : α → Prop) (h₁ : ∃ x, P x)
+(h₂ : ∀ x, P x → Q x) : ∃ x, Q x :=
+by do (dir, goals) ← create_directory,
+  trace_directory dir,
+  mi ← create_match_info dir goals,
+  trace_match_info mi, -- the important line
+
+  t₁ ← get_local `h₁,
+  nmx ← get_unused_name `x,
+  nmh ← get_unused_name `h,
+  cases t₁ [nmx, nmh],
+  x ← get_local nmx,
+  h ← get_local nmh,
+  applyc ``exists.intro,
+  t₂ ← get_local `h₂,
+  apply t₂,
+  exact h
